Revise semantics of assignment w.r.t. the return value of an assignment
The value of `lhs = rhs` used to be the value of `rhs` cast to the
type of `lhs`.  This is incorrect if `lhs` denotes a bitfield in a
struct or union.  E.g. if `int f: 2`, `x.f = 7` evaluates to `-1`, not `7`.

In this commit we modify `assign_loc` and `store_bitfield` to return
the value of the assignment expression.  We use this in the semantics
of assignment expressions in Csem.

We then adapt SimplExpr to the revised semantics of assignment return
values.  The generated Clight code now correctly zero- or sign-extends
the assigned value if the lhs is a bitfield.

cfrontend/Cexec.v
@@ -37,6 +37,10 @@ Notation "'do' X , Y , Z <- A ; B" := (match A with Some (X, Y, Z) => B | None =
   (at level 200, X ident, Y ident, Z ident, A at level 100, B at level 200)
   : option_monad_scope.
 
+Notation "'do' X , Y , Z , W <- A ; B" := (match A with Some (X, Y, Z, W) => B | None => None end)
+  (at level 200, X ident, Y ident, Z ident, W ident, A at level 100, B at level 200)
+  : option_monad_scope.
+
 Notation " 'check' A ; B" := (if A then B else None)
   (at level 200, A at level 100, B at level 200)
   : option_monad_scope.
@@ -209,15 +213,15 @@ Definition do_volatile_load (w: world) (chunk: memory_chunk) (m: mem) (b: block)
     Some(w, E0, v).
 
 Definition do_volatile_store (w: world) (chunk: memory_chunk) (m: mem) (b: block) (ofs: ptrofs) (v: val)
-                             : option (world * trace * mem) :=
+                             : option (world * trace * mem * val) :=
   if Genv.block_is_volatile ge b then
     do id <- Genv.invert_symbol ge b;
     do ev <- eventval_of_val (Val.load_result chunk v) (type_of_chunk chunk);
     do w' <- nextworld_vstore w chunk id ofs ev;
-    Some(w', Event_vstore chunk id ofs ev :: nil, m)
+    Some(w', Event_vstore chunk id ofs ev :: nil, m, v)
   else
     do m' <- Mem.store chunk m b (Ptrofs.unsigned ofs) v;
-    Some(w, E0, m').
+    Some(w, E0, m', v).
 
 Lemma do_volatile_load_sound:
   forall w chunk m b ofs w' t v,
@@ -244,21 +248,21 @@ Proof.
 Qed.
 
 Lemma do_volatile_store_sound:
-  forall w chunk m b ofs v w' t m',
-  do_volatile_store w chunk m b ofs v = Some(w', t, m') ->
-  volatile_store ge chunk m b ofs v t m' /\ possible_trace w t w'.
+  forall w chunk m b ofs v w' t m' v',
+  do_volatile_store w chunk m b ofs v = Some(w', t, m', v') ->
+  volatile_store ge chunk m b ofs v t m' /\ possible_trace w t w' /\ v' = v.
 Proof.
-  intros until m'. unfold do_volatile_store. mydestr.
+  intros until v'. unfold do_volatile_store. mydestr.
   split. constructor; auto. apply Genv.invert_find_symbol; auto.
   apply eventval_of_val_sound; auto.
-  econstructor. constructor; eauto. constructor.
-  split. constructor; auto. constructor.
+  split. econstructor. constructor; eauto. constructor. auto.
+  split. constructor; auto. split. constructor. auto.
 Qed.
 
 Lemma do_volatile_store_complete:
   forall w chunk m b ofs v w' t m',
   volatile_store ge chunk m b ofs v t m' -> possible_trace w t w' ->
-  do_volatile_store w chunk m b ofs v = Some(w', t, m').
+  do_volatile_store w chunk m b ofs v = Some(w', t, m', v).
 Proof.
   unfold do_volatile_store; intros. inv H; simpl in *.
   rewrite H1. rewrite (Genv.find_invert_symbol _ _ H2).
@@ -326,13 +330,13 @@ Proof with try (right; intuition lia).
   destruct Y... left; intuition lia.
 Defined.
 
-Definition do_assign_loc (w: world) (ty: type) (m: mem) (b: block) (ofs: ptrofs) (bf: bitfield) (v: val): option (world * trace * mem) :=
+Definition do_assign_loc (w: world) (ty: type) (m: mem) (b: block) (ofs: ptrofs) (bf: bitfield) (v: val): option (world * trace * mem * val) :=
   match bf with
   | Full =>
     match access_mode ty with
     | By_value chunk =>
         match type_is_volatile ty with
-        | false => do m' <- Mem.storev chunk m (Vptr b ofs) v; Some(w, E0, m')
+        | false => do m' <- Mem.storev chunk m (Vptr b ofs) v; Some(w, E0, m', v)
         | true => do_volatile_store w chunk m b ofs v
         end
     | By_copy =>
@@ -341,7 +345,7 @@ Definition do_assign_loc (w: world) (ty: type) (m: mem) (b: block) (ofs: ptrofs)
             if check_assign_copy ty b ofs b' ofs' then
               do bytes <- Mem.loadbytes m b' (Ptrofs.unsigned ofs') (sizeof ge ty);
               do m' <- Mem.storebytes m b (Ptrofs.unsigned ofs) bytes;
-              Some(w, E0, m')
+              Some(w, E0, m', v)
             else None
         | _ => None
         end
@@ -350,12 +354,14 @@ Definition do_assign_loc (w: world) (ty: type) (m: mem) (b: block) (ofs: ptrofs)
   | Bits sz sg pos width =>
     check (negb (type_is_volatile ty));
     check (zle 0 pos && zlt 0 width && zle (pos + width) (bitsize_intsize sz));
-    match v, Mem.loadv (chunk_for_carrier sz) m (Vptr b ofs) with
-    | Vint n, Some (Vint c) =>
+    match ty, v, Mem.loadv (chunk_for_carrier sz) m (Vptr b ofs) with
+    | Tint sz1 sg1 _, Vint n, Some (Vint c) =>
+        check (intsize_eq sz1 sz &&
+               signedness_eq sg1 (if zlt width (bitsize_intsize sz) then Signed else sg));
         do m' <- Mem.storev (chunk_for_carrier sz) m (Vptr b ofs)
                             (Vint ((Int.bitfield_insert (first_bit sz pos width) width c n)));
-        Some (w, E0, m')
-    | _, _ => None
+        Some (w, E0, m', Vint (bitfield_normalize sz sg width n))
+    | _, _, _ => None
     end
   end.
 
@@ -392,26 +398,26 @@ Proof.
 Qed.
 
 Lemma do_assign_loc_sound:
-  forall w ty m b ofs bf v w' t m',
-  do_assign_loc w ty m b ofs bf v = Some(w', t, m') ->
-  assign_loc ge ty m b ofs bf v t m' /\ possible_trace w t w'.
+  forall w ty m b ofs bf v w' t m' v',
+  do_assign_loc w ty m b ofs bf v = Some(w', t, m', v') ->
+  assign_loc ge ty m b ofs bf v t m' v' /\ possible_trace w t w'.
 Proof.
-  unfold do_assign_loc; intros until m'.
+  unfold do_assign_loc; intros until v'.
   destruct bf.
 - destruct (access_mode ty) eqn:?; mydestr.
-  intros. exploit do_volatile_store_sound; eauto. intuition. eapply assign_loc_volatile; eauto.
+  intros. exploit do_volatile_store_sound; eauto. intros (P & Q & R). subst v'. intuition. eapply assign_loc_volatile; eauto.
   split. eapply assign_loc_value; eauto. constructor.
   destruct v; mydestr. destruct a as [P [Q R]].
   split. eapply assign_loc_copy; eauto. constructor.
 - mydestr. apply negb_true_iff in Heqb0. InvBooleans.
-  destruct v; mydestr. destruct v; mydestr. 
+  destruct ty; mydestr. destruct v; mydestr. destruct v; mydestr. InvBooleans. subst s i.
   split. eapply assign_loc_bitfield; eauto. econstructor; eauto. constructor.
 Qed.
 
 Lemma do_assign_loc_complete:
-  forall w ty m b ofs bf v w' t m',
-  assign_loc ge ty m b ofs bf v t m' -> possible_trace w t w' ->
-  do_assign_loc w ty m b ofs bf v = Some(w', t, m').
+  forall w ty m b ofs bf v w' t m' v',
+  assign_loc ge ty m b ofs bf v t m' v' -> possible_trace w t w' ->
+  do_assign_loc w ty m b ofs bf v = Some(w', t, m', v').
 Proof.
   unfold do_assign_loc; intros. inv H.
 - inv H0. rewrite H1; rewrite H2; rewrite H3; auto.
@@ -421,7 +427,8 @@ Proof.
   elim n. red; tauto.
 - inv H0. inv H2. rewrite H1; simpl. 
   unfold proj_sumbool; rewrite ! zle_true, ! zlt_true by lia. cbn.
-  cbn in H4; rewrite H4. cbn in H5; rewrite H5. auto.
+  rewrite ! dec_eq_true.
+  cbn in H5; rewrite H5. cbn in H6; rewrite H6. auto.
 Qed.
 
 (** External calls *)
@@ -464,7 +471,7 @@ Definition do_ef_volatile_load (chunk: memory_chunk)
 Definition do_ef_volatile_store (chunk: memory_chunk)
        (w: world) (vargs: list val) (m: mem) : option (world * trace * val * mem) :=
   match vargs with
-  | Vptr b ofs :: v :: nil => do w',t,m' <- do_volatile_store w chunk m b ofs v; Some(w',t,Vundef,m')
+  | Vptr b ofs :: v :: nil => do w',t,m',v' <- do_volatile_store w chunk m b ofs v; Some(w',t,Vundef,m')
   | _ => None
   end.
 
@@ -607,7 +614,7 @@ Proof with try congruence.
   exploit do_volatile_load_sound; eauto. intuition. econstructor; eauto.
 - (* EF_vstore *)
   unfold do_ef_volatile_store. destruct vargs... destruct v... destruct vargs... destruct vargs...
-  mydestr. destruct p as [[w'' t''] m'']. mydestr.
+  mydestr. destruct p as [[[w'' t''] m''] v'']. mydestr.
   exploit do_volatile_store_sound; eauto. intuition. econstructor; eauto.
 - (* EF_malloc *)
   unfold do_ef_malloc. destruct vargs... destruct vargs... mydestr.
@@ -753,6 +760,10 @@ Notation "'do' X , Y , Z <- A ; B" := (match A with Some (X, Y, Z) => B | None =
   (at level 200, X ident, Y ident, Z ident, A at level 100, B at level 200)
   : reducts_monad_scope.
 
+Notation "'do' X , Y , Z , W <- A ; B" := (match A with Some (X, Y, Z, W) => B | None => stuck end)
+  (at level 200, X ident, Y ident, Z ident, W ident, A at level 100, B at level 200)
+  : reducts_monad_scope.
+
 Notation " 'check' A ; B" := (if A then B else stuck)
   (at level 200, A at level 100, B at level 200)
   : reducts_monad_scope.
@@ -883,8 +894,8 @@ Fixpoint step_expr (k: kind) (a: expr) (m: mem): reducts expr :=
       | Some(b, ofs, bf, ty1), Some(v2, ty2) =>
           check type_eq ty1 ty;
           do v <- sem_cast v2 ty2 ty1 m;
-          do w',t,m' <- do_assign_loc w ty1 m b ofs bf v;
-          topred (Rred "red_assign" (Eval v ty) m' t)
+          do w',t,m',v' <- do_assign_loc w ty1 m b ofs bf v;
+          topred (Rred "red_assign" (Eval v' ty) m' t)
       | _, _ =>
          incontext2 (fun x => Eassign x r2 ty) (step_expr LV l1 m)
                     (fun x => Eassign l1 x ty) (step_expr RV r2 m)
@@ -1042,8 +1053,8 @@ Definition invert_expr_prop (a: expr) (m: mem) : Prop :=
   | Econdition (Eval v1 ty1) r1 r2 ty =>
       exists b, bool_val v1 ty1 m = Some b
   | Eassign (Eloc b ofs bf ty1) (Eval v2 ty2) ty =>
-      exists v, exists m', exists t, exists w',
-      ty = ty1 /\ sem_cast v2 ty2 ty1 m = Some v /\ assign_loc ge ty1 m b ofs bf v t m' /\ possible_trace w t w'
+      exists v, exists m', exists v', exists t, exists w',
+      ty = ty1 /\ sem_cast v2 ty2 ty1 m = Some v /\ assign_loc ge ty1 m b ofs bf v t m' v' /\ possible_trace w t w'
   | Eassignop op (Eloc b ofs bf ty1) (Eval v2 ty2) tyres ty =>
       exists t, exists v1, exists w',
       ty = ty1 /\ deref_loc ge ty1 m b ofs bf t v1 /\ possible_trace w t w'
@@ -1092,7 +1103,7 @@ Proof.
   exists true; auto. exists false; auto.
   exists true; auto. exists false; auto.
   exists b; auto.
-  exists v; exists m'; exists t; exists w'; auto.
+  exists v; exists m'; exists v'; exists t; exists w'; auto.
   exists t; exists v1; exists w'; auto.
   exists t; exists v1; exists w'; auto.
   exists v; auto.
@@ -1509,9 +1520,9 @@ Proof with (try (apply not_invert_ok; simpl; intro; myinv; intuition congruence;
   (* top *)
   destruct (type_eq ty1 ty)... subst ty1.
   destruct (sem_cast v2 ty2 ty m) as [v|] eqn:?...
-  destruct (do_assign_loc w ty m b ofs bf v) as [[[w' t] m']|] eqn:?.
+  destruct (do_assign_loc w ty m b ofs bf v) as [[[[w' t] m'] v']|] eqn:?.
   exploit do_assign_loc_sound; eauto. intros [P Q].
-  apply topred_ok; auto. split. apply red_assign; auto. exists w'; auto.
+  apply topred_ok; auto. split. eapply red_assign; eauto. exists w'; auto.
   apply not_invert_ok; simpl; intros; myinv. exploit do_assign_loc_complete; eauto. congruence.
   (* depth *)
   eapply incontext2_ok; eauto.
@@ -1662,7 +1673,7 @@ Proof.
 (* alignof *)
   inv H. econstructor; eauto.
 (* assign *)
-  rewrite dec_eq_true. rewrite H. rewrite (do_assign_loc_complete _ _ _ _ _ _ _ _ _ _ H0 H1).
+  rewrite dec_eq_true. rewrite H. rewrite (do_assign_loc_complete _ _ _ _ _ _ _ _ _ _ _ H0 H1).
   econstructor; eauto.
 (* assignop *)
   rewrite dec_eq_true. rewrite (do_deref_loc_complete _ _ _ _ _ _ _ _ _ H H0).
@@ -1968,7 +1979,7 @@ Function sem_bind_parameters (w: world) (e: env) (m: mem) (l: list (ident * type
       match PTree.get id e with
          | Some (b, ty') =>
              check (type_eq ty ty');
-             do w', t, m1 <- do_assign_loc w ty m b Ptrofs.zero Full v1;
+             do w', t, m1, v' <- do_assign_loc w ty m b Ptrofs.zero Full v1;
              match t with nil => sem_bind_parameters w e m1 params lv | _ => None end
         | None => None
       end
@@ -1992,7 +2003,7 @@ Local Opaque do_assign_loc.
    induction 1; simpl; auto.
    rewrite H. rewrite dec_eq_true.
    assert (possible_trace w E0 w) by constructor.
-   rewrite (do_assign_loc_complete _ _ _ _ _ _ _ _ _ _ H0 H2).
+   rewrite (do_assign_loc_complete _ _ _ _ _ _ _ _ _ _ _ H0 H2).
    simpl. auto.
 Qed.
 
