cfrontend/Cstrategy.v
@@ -282,28 +282,28 @@ Inductive estep: state -> trace -> state -> Prop :=
       estep (ExprState f (C (Econdition r1 r2 r3 ty)) k e m)
          E0 (ExprState f (C (Eparen (if b then r2 else r3) ty ty)) k e m)
 
-  | step_assign: forall f C l r ty k e m b ofs bf v v' t m',
+  | step_assign: forall f C l r ty k e m b ofs bf v v1 t m' v',
       leftcontext RV RV C ->
       eval_simple_lvalue e m l b ofs bf ->
       eval_simple_rvalue e m r v ->
-      sem_cast v (typeof r) (typeof l) m = Some v' ->
-      assign_loc ge (typeof l) m b ofs bf v' t m' ->
+      sem_cast v (typeof r) (typeof l) m = Some v1 ->
+      assign_loc ge (typeof l) m b ofs bf v1 t m' v' ->
       ty = typeof l ->
       estep (ExprState f (C (Eassign l r ty)) k e m)
           t (ExprState f (C (Eval v' ty)) k e m')
 
-  | step_assignop: forall f C op l r tyres ty k e m b ofs bf v1 v2 v3 v4 t1 t2 m' t,
+  | step_assignop: forall f C op l r tyres ty k e m b ofs bf v1 v2 v3 v4 t1 t2 m' v' t,
       leftcontext RV RV C ->
       eval_simple_lvalue e m l b ofs bf ->
       deref_loc ge (typeof l) m b ofs bf t1 v1 ->
       eval_simple_rvalue e m r v2 ->
       sem_binary_operation ge op v1 (typeof l) v2 (typeof r) m = Some v3 ->
       sem_cast v3 tyres (typeof l) m = Some v4 ->
-      assign_loc ge (typeof l) m b ofs bf v4 t2 m' ->
+      assign_loc ge (typeof l) m b ofs bf v4 t2 m' v' ->
       ty = typeof l ->
       t = t1 ** t2 ->
       estep (ExprState f (C (Eassignop op l r tyres ty)) k e m)
-          t (ExprState f (C (Eval v4 ty)) k e m')
+          t (ExprState f (C (Eval v' ty)) k e m')
 
   | step_assignop_stuck: forall f C op l r tyres ty k e m b ofs bf v1 v2 t,
       leftcontext RV RV C ->
@@ -315,20 +315,20 @@ Inductive estep: state -> trace -> state -> Prop :=
       | Some v3 =>
           match sem_cast v3 tyres (typeof l) m with
           | None => True
-          | Some v4 => forall t2 m', ~(assign_loc ge (typeof l) m b ofs bf v4 t2 m')
+          | Some v4 => forall t2 m' v', ~(assign_loc ge (typeof l) m b ofs bf v4 t2 m' v')
           end
       end ->
       ty = typeof l ->
       estep (ExprState f (C (Eassignop op l r tyres ty)) k e m)
           t Stuckstate
 
-  | step_postincr: forall f C id l ty k e m b ofs bf v1 v2 v3 t1 t2 m' t,
+  | step_postincr: forall f C id l ty k e m b ofs bf v1 v2 v3 t1 t2 m' v' t,
       leftcontext RV RV C ->
       eval_simple_lvalue e m l b ofs bf ->
       deref_loc ge ty m b ofs bf t1 v1 ->
       sem_incrdecr ge id v1 ty m = Some v2 ->
       sem_cast v2 (incrdecr_type ty) ty m = Some v3 ->
-      assign_loc ge ty m b ofs bf v3 t2 m' ->
+      assign_loc ge ty m b ofs bf v3 t2 m' v' ->
       ty = typeof l ->
       t = t1 ** t2 ->
       estep (ExprState f (C (Epostincr id l ty)) k e m)
@@ -343,7 +343,7 @@ Inductive estep: state -> trace -> state -> Prop :=
       | Some v2 =>
           match sem_cast v2 (incrdecr_type ty) ty m with
           | None => True
-          | Some v3 => forall t2 m', ~(assign_loc ge (typeof l) m b ofs bf v3 t2 m')
+          | Some v3 => forall t2 m' v', ~(assign_loc ge (typeof l) m b ofs bf v3 t2 m' v')
           end
       end ->
       ty = typeof l ->
@@ -551,14 +551,14 @@ Definition invert_expr_prop (a: expr) (m: mem) : Prop :=
   | Econdition (Eval v1 ty1) r1 r2 ty =>
       exists b, bool_val v1 ty1 m = Some b
   | Eassign (Eloc b ofs bf ty1) (Eval v2 ty2) ty =>
-      exists v, exists m', exists t,
-      ty = ty1 /\ sem_cast v2 ty2 ty1 m = Some v /\ assign_loc ge ty1 m b ofs bf v t m'
+      exists v m' v' t,
+      ty = ty1 /\ sem_cast v2 ty2 ty1 m = Some v /\ assign_loc ge ty1 m b ofs bf v t m' v'
   | Eassignop op (Eloc b ofs bf ty1) (Eval v2 ty2) tyres ty =>
-      exists t, exists v1,
+      exists t v1,
       ty = ty1
       /\ deref_loc ge ty1 m b ofs bf t v1
   | Epostincr id (Eloc b ofs bf ty1) ty =>
-      exists t, exists v1,
+      exists t v1,
       ty = ty1
       /\ deref_loc ge ty m b ofs bf t v1
   | Ecomma (Eval v ty1) r2 ty =>
@@ -602,7 +602,7 @@ Proof.
   exists true; auto. exists false; auto.
   exists true; auto. exists false; auto.
   exists b; auto.
-  exists v; exists m'; exists t; auto.
+  exists v; exists m'; exists v'; exists t; auto.
   exists t; exists v1; auto.
   exists t; exists v1; auto.
   exists v; auto.
@@ -1209,7 +1209,7 @@ Proof.
   left; apply step_rred with (C := fun x => C(Eassign (Eloc b ofs bf (typeof l)) x (typeof l))); eauto. econstructor; eauto.
   apply star_one.
   left; eapply step_stuck; eauto.
-  red; intros. exploit imm_safe_inv; eauto. simpl. intros [v4' [m' [t' [A [B D]]]]].
+  red; intros. exploit imm_safe_inv; eauto. simpl. intros [v4' [m' [v' [t' [A [B D]]]]]].
   rewrite B in H4. eelim H4; eauto.
   reflexivity.
   apply star_one.
@@ -1246,7 +1246,7 @@ Proof.
   econstructor; eauto.
   apply star_one.
   left; eapply step_stuck with (C := fun x => C (Ecomma x (Eval v1 (typeof l)) (typeof l))); eauto.
-  red; intros. exploit imm_safe_inv; eauto. simpl. intros [v3 [m' [t' [A [B D]]]]].
+  red; intros. exploit imm_safe_inv; eauto. simpl. intros [v3 [m' [v' [t' [A [B D]]]]]].
   rewrite B in H3. eelim H3; eauto.
   reflexivity.
   apply star_one.
@@ -1323,7 +1323,7 @@ Proof.
   intros (b & ofs & bf & E1 & S1).
   exploit (simple_can_eval_rval f k e m b2 (fun x => C(Eassign (Eloc b ofs bf (typeof b1)) x ty))); eauto.
   intros [v [E2 S2]].
-  exploit safe_inv. eexact S2. eauto. simpl. intros [v' [m' [t [A [B D]]]]].
+  exploit safe_inv. eexact S2. eauto. simpl. intros [v1 [m' [v' [t [A [B D]]]]]].
   econstructor; econstructor; eapply step_assign; eauto.
 (* assignop *)
   destruct Q.
@@ -1334,11 +1334,11 @@ Proof.
   exploit safe_inv. eexact S2. eauto. simpl. intros [t1 [v1 [A B]]].
   destruct (sem_binary_operation ge op v1 (typeof b1) v (typeof b2) m) as [v3|] eqn:?.
   destruct (sem_cast v3 tyres (typeof b1) m) as [v4|] eqn:?.
-  destruct (classic (exists t2, exists m', assign_loc ge (typeof b1) m b ofs bf v4 t2 m')).
-  destruct H2 as [t2 [m' D]].
+  destruct (classic (exists t2 m' v', assign_loc ge (typeof b1) m b ofs bf v4 t2 m' v')).
+  destruct H2 as [t2 [m' [v' D]]].
   econstructor; econstructor; eapply step_assignop; eauto.
   econstructor; econstructor; eapply step_assignop_stuck; eauto.
-  rewrite Heqo. rewrite Heqo0. intros; red; intros. elim H2. exists t2; exists m'; auto.
+  rewrite Heqo. rewrite Heqo0. intros; red; intros. elim H2. exists t2, m', v'; auto.
   econstructor; econstructor; eapply step_assignop_stuck; eauto.
   rewrite Heqo. rewrite Heqo0. auto.
   econstructor; econstructor; eapply step_assignop_stuck; eauto.
@@ -1349,11 +1349,11 @@ Proof.
   exploit safe_inv. eexact S1. eauto. simpl. intros [t [v1 [A B]]].
   destruct (sem_incrdecr ge id v1 ty m) as [v2|] eqn:?.
   destruct (sem_cast v2 (incrdecr_type ty) ty m) as [v3|] eqn:?.
-  destruct (classic (exists t2, exists m', assign_loc ge ty m b1 ofs bf v3 t2 m')).
-  destruct H0 as [t2 [m' D]].
+  destruct (classic (exists t2 m' v', assign_loc ge ty m b1 ofs bf v3 t2 m' v')).
+  destruct H0 as [t2 [m' [v' D]]].
   econstructor; econstructor; eapply step_postincr; eauto.
   econstructor; econstructor; eapply step_postincr_stuck; eauto.
-  rewrite Heqo. rewrite Heqo0. intros; red; intros. elim H0. exists t2; exists m'; congruence.
+  rewrite Heqo. rewrite Heqo0. intros; red; intros. elim H0. exists t2, m', v'; congruence.
   econstructor; econstructor; eapply step_postincr_stuck; eauto.
   rewrite Heqo. rewrite Heqo0. auto.
   econstructor; econstructor; eapply step_postincr_stuck; eauto.
@@ -1464,16 +1464,16 @@ Proof.
 Qed.
 
 Remark assign_loc_trace:
-  forall ge ty m b ofs bf t v m',
-  assign_loc ge ty m b ofs bf v t m' ->
+  forall ge ty m b ofs bf t v m' v',
+  assign_loc ge ty m b ofs bf v t m' v' ->
   match t with nil => True | ev :: nil => output_event ev | _ => False end.
 Proof.
   intros. inv H; simpl; auto. inv H2; simpl; auto.
 Qed.
 
 Remark assign_loc_receptive:
-  forall ge ty m b ofs bf ev1 t1 v m' ev2,
-  assign_loc ge ty m b ofs bf v (ev1 :: t1) m' ->
+  forall ge ty m b ofs bf ev1 t1 v m' v' ev2,
+  assign_loc ge ty m b ofs bf v (ev1 :: t1) m' v' ->
   match_traces ge (ev1 :: nil) (ev2 :: nil) ->
   ev1 :: t1 = ev2 :: nil.
 Proof.
@@ -1503,11 +1503,11 @@ Proof.
   inv H10. exploit deref_loc_receptive; eauto. intros [EQ [v1' A]]. subst t0.
   destruct (sem_binary_operation ge op v1' (typeof l) v2 (typeof r) m) as [v3'|] eqn:?.
   destruct (sem_cast v3' tyres (typeof l) m) as [v4'|] eqn:?.
-  destruct (classic (exists t2', exists m'', assign_loc ge (typeof l) m b ofs bf v4' t2' m'')).
-  destruct H1 as [t2' [m'' P]].
+  destruct (classic (exists t2' m'' v'', assign_loc ge (typeof l) m b ofs bf v4' t2' m'' v'')).
+  destruct H1 as [t2' [m'' [v'' P]]].
   econstructor; econstructor. left; eapply step_assignop with (v1 := v1'); eauto. simpl; reflexivity.
   econstructor; econstructor. left; eapply step_assignop_stuck with (v1 := v1'); eauto.
-  rewrite Heqo; rewrite Heqo0. intros; red; intros; elim H1. exists t0; exists m'0; auto.
+  rewrite Heqo; rewrite Heqo0. intros; red; intros; elim H1. exists t0, m'0, v'0; auto.
   econstructor; econstructor. left; eapply step_assignop_stuck with (v1 := v1'); eauto.
   rewrite Heqo; rewrite Heqo0; auto.
   econstructor; econstructor. left; eapply step_assignop_stuck with (v1 := v1'); eauto.
@@ -1516,11 +1516,11 @@ Proof.
   exploit deref_loc_receptive; eauto. intros [EQ [v1' A]]. subst t1.
   destruct (sem_binary_operation ge op v1' (typeof l) v2 (typeof r) m) as [v3'|] eqn:?.
   destruct (sem_cast v3' tyres (typeof l) m) as [v4'|] eqn:?.
-  destruct (classic (exists t2', exists m'', assign_loc ge (typeof l) m b ofs bf v4' t2' m'')).
-  destruct H1 as [t2' [m'' P]].
+  destruct (classic (exists t2' m'' v'', assign_loc ge (typeof l) m b ofs bf v4' t2' m'' v'')).
+  destruct H1 as [t2' [m'' [v'' P]]].
   econstructor; econstructor. left; eapply step_assignop with (v1 := v1'); eauto. simpl; reflexivity.
   econstructor; econstructor. left; eapply step_assignop_stuck with (v1 := v1'); eauto.
-  rewrite Heqo; rewrite Heqo0. intros; red; intros; elim H1. exists t2; exists m'; auto.
+  rewrite Heqo; rewrite Heqo0. intros; red; intros; elim H1. exists t2, m', v'; auto.
   econstructor; econstructor. left; eapply step_assignop_stuck with (v1 := v1'); eauto.
   rewrite Heqo; rewrite Heqo0; auto.
   econstructor; econstructor. left; eapply step_assignop_stuck with (v1 := v1'); eauto.
@@ -1532,11 +1532,11 @@ Proof.
   inv H9. exploit deref_loc_receptive; eauto. intros [EQ [v1' A]]. subst t0.
   destruct (sem_incrdecr ge id v1' (typeof l) m) as [v2'|] eqn:?.
   destruct (sem_cast v2' (incrdecr_type (typeof l)) (typeof l) m) as [v3'|] eqn:?.
-  destruct (classic (exists t2', exists m'', assign_loc ge (typeof l) m b ofs bf v3' t2' m'')).
-  destruct H1 as [t2' [m'' P]].
+  destruct (classic (exists t2' m'' v'', assign_loc ge (typeof l) m b ofs bf v3' t2' m'' v'')).
+  destruct H1 as [t2' [m'' [v'' P]]].
   econstructor; econstructor. left; eapply step_postincr with (v1 := v1'); eauto. simpl; reflexivity.
   econstructor; econstructor. left; eapply step_postincr_stuck with (v1 := v1'); eauto.
-  rewrite Heqo; rewrite Heqo0. intros; red; intros; elim H1. exists t0; exists m'0; auto.
+  rewrite Heqo; rewrite Heqo0. intros; red; intros; elim H1. exists t0, m'0, v'0; auto.
   econstructor; econstructor. left; eapply step_postincr_stuck with (v1 := v1'); eauto.
   rewrite Heqo; rewrite Heqo0; auto.
   econstructor; econstructor. left; eapply step_postincr_stuck with (v1 := v1'); eauto.
@@ -1545,11 +1545,11 @@ Proof.
   exploit deref_loc_receptive; eauto. intros [EQ [v1' A]]. subst t1.
   destruct (sem_incrdecr ge id v1' (typeof l) m) as [v2'|] eqn:?.
   destruct (sem_cast v2' (incrdecr_type (typeof l)) (typeof l) m) as [v3'|] eqn:?.
-  destruct (classic (exists t2', exists m'', assign_loc ge (typeof l) m b ofs bf v3' t2' m'')).
-  destruct H1 as [t2' [m'' P]].
+  destruct (classic (exists t2' m'' v'', assign_loc ge (typeof l) m b ofs bf v3' t2' m'' v'')).
+  destruct H1 as [t2' [m'' [v'' P]]].
   econstructor; econstructor. left; eapply step_postincr with (v1 := v1'); eauto. simpl; reflexivity.
   econstructor; econstructor. left; eapply step_postincr_stuck with (v1 := v1'); eauto.
-  rewrite Heqo; rewrite Heqo0. intros; red; intros; elim H1. exists t2; exists m'; auto.
+  rewrite Heqo; rewrite Heqo0. intros; red; intros; elim H1. exists t2, m', v'; auto.
   econstructor; econstructor. left; eapply step_postincr_stuck with (v1 := v1'); eauto.
   rewrite Heqo; rewrite Heqo0; auto.
   econstructor; econstructor. left; eapply step_postincr_stuck with (v1 := v1'); eauto.
@@ -1727,32 +1727,32 @@ with eval_expr: env -> mem -> kind -> expr -> trace -> mem -> expr -> Prop :=
       eval_expr e m RV (Esizeof ty' ty) E0 m (Esizeof ty' ty)
   | eval_alignof: forall e m ty' ty,
       eval_expr e m RV (Ealignof ty' ty) E0 m (Ealignof ty' ty)
-  | eval_assign: forall e m l r ty t1 m1 l' t2 m2 r' b ofs bf v v' t3 m3,
+  | eval_assign: forall e m l r ty t1 m1 l' t2 m2 r' b ofs bf v v1 v' t3 m3,
       eval_expr e m LV l t1 m1 l' -> eval_expr e m1 RV r t2 m2 r' ->
       eval_simple_lvalue ge e m2 l' b ofs bf ->
       eval_simple_rvalue ge e m2 r' v ->
-      sem_cast v (typeof r) (typeof l) m2 = Some v' ->
-      assign_loc ge (typeof l) m2 b ofs bf v' t3 m3 ->
+      sem_cast v (typeof r) (typeof l) m2 = Some v1 ->
+      assign_loc ge (typeof l) m2 b ofs bf v1 t3 m3 v' ->
       ty = typeof l ->
       eval_expr e m RV (Eassign l r ty) (t1**t2**t3) m3 (Eval v' ty)
   | eval_assignop: forall e m op l r tyres ty t1 m1 l' t2 m2 r' b ofs bf
-                          v1 v2 v3 v4 t3 t4 m3,
+                          v1 v2 v3 v4 v' t3 t4 m3,
       eval_expr e m LV l t1 m1 l' -> eval_expr e m1 RV r t2 m2 r' ->
       eval_simple_lvalue ge e m2 l' b ofs bf ->
       deref_loc ge (typeof l) m2 b ofs bf t3 v1 ->
       eval_simple_rvalue ge e m2 r' v2 ->
       sem_binary_operation ge op v1 (typeof l) v2 (typeof r) m2 = Some v3 ->
       sem_cast v3 tyres (typeof l) m2 = Some v4 ->
-      assign_loc ge (typeof l) m2 b ofs bf v4 t4 m3 ->
+      assign_loc ge (typeof l) m2 b ofs bf v4 t4 m3 v' ->
       ty = typeof l ->
-      eval_expr e m RV (Eassignop op l r tyres ty) (t1**t2**t3**t4) m3 (Eval v4 ty)
-  | eval_postincr: forall e m id l ty t1 m1 l' b ofs bf v1 v2 v3 m2 t2 t3,
+      eval_expr e m RV (Eassignop op l r tyres ty) (t1**t2**t3**t4) m3 (Eval v' ty)
+  | eval_postincr: forall e m id l ty t1 m1 l' b ofs bf v1 v2 v3 v' m2 t2 t3,
       eval_expr e m LV l t1 m1 l' ->
       eval_simple_lvalue ge e m1 l' b ofs bf ->
       deref_loc ge ty m1 b ofs bf t2 v1 ->
       sem_incrdecr ge id v1 ty m1 = Some v2 ->
       sem_cast v2 (incrdecr_type ty) ty m1 = Some v3 ->
-      assign_loc ge ty m1 b ofs bf v3 t3 m2 ->
+      assign_loc ge ty m1 b ofs bf v3 t3 m2 v' ->
       ty = typeof l ->
       eval_expr e m RV (Epostincr id l ty) (t1**t2**t3) m2 (Eval v1 ty)
   | eval_comma: forall e m r1 r2 ty t1 m1 r1' v1 t2 m2 r2',
@@ -2315,7 +2315,7 @@ Proof.
   simpl; intuition.
   eapply star_trans. eexact D.
   eapply star_right. eexact G.
-  left. eapply step_assign; eauto. congruence. rewrite B; eauto. congruence.
+  left. eapply step_assign with (v1 := v1); eauto. congruence. rewrite B; eauto. congruence.
   reflexivity. traceEq.
 (* assignop *)
   exploit (H0 (fun x => C(Eassignop op x r tyres ty))).
@@ -2326,7 +2326,7 @@ Proof.
   eapply star_trans. eexact D.
   eapply star_right. eexact G.
   left. eapply step_assignop; eauto.
-  rewrite B; eauto. rewrite B; rewrite F; eauto. congruence. rewrite B; eauto. congruence.
+  rewrite B; eauto. rewrite B; rewrite F; eauto. rewrite B; eauto. rewrite B; eauto. congruence.
   reflexivity. traceEq.
 (* postincr *)
   exploit (H0 (fun x => C(Epostincr id x ty))).
